L_Core_Soundness.v
@@ -20,8 +20,8 @@ Scheme typing_prf_ind := Induction for typing_prf Sort Prop
                        with typing_clos_ind := Induction for typing_clos Sort Prop.
 About typing_clos_ind.
 
-Combined Scheme typing_mutind from typing_prf_ind,typing_cont_ind,typing_clos_ind.
-About typing_mutind.
+Combined Scheme typing_mut_ind from typing_prf_ind,typing_cont_ind,typing_clos_ind.
+
 Lemma typing_weaken :
   (  forall A p  T (H: A|= p :+ T) E F G,
        A=E&G -> 
@@ -31,7 +31,7 @@ A=E&G ->  ok (E & F & G) ->   (E & F & G) |= e :- T)
 /\ (forall A c  (H: (c:* A)) E F G,
  A=E&G -> ok (E & F & G) ->   c:* (E & F & G)) .
 Proof.
-  apply (typing_mutind ).
+  apply (typing_mut_ind ).
   + intros A a T OkA Binds E F G HA Ok.
     apply* typing_prf_var. apply* binds_weaken.
     rewrite HA in Binds.
@@ -96,70 +96,235 @@ Proof.
 Qed.
 
 (** Typing is preserved by substitution. *)
-
-  
-Fixpoint typing_subst_prf F U E p T z q (H:(E & z ~ pos U & F) |= p:+ T) {struct H}:
-  E |= q :+ U -> (E & F) |= [z ~+> q]+ p :+ T
-with typing_subst_cont F U E e T z q (H:(E & z ~ pos U & F) |= e:- T ) {struct H}:
-   E |= q :+ U -> (E & F) |= [z ~+> q]- e :- T
-with typing_subst_clos F U E c z q (H:c:* (E & z ~ pos U & F)) {struct H}:
-   E |= q :+ U -> [z ~+> q]* c :* (E&F).
+About typing_mut_ind.
+Lemma typing_subst_prf:
+  (forall  A  p T (H: A |= p:+ T) F U E z q,
+     A=(E & z ~ pos U & F) -> E |= q :+ U -> (E & F) |= [z ~+> q]+ p :+ T)
+  /\(forall A e T (H: A |= e:- T ) F U E z q,
+   A=(E & z ~ pos U & F)   ->   E |= q :+ U -> (E & F) |= [z ~+> q]- e :- T)
+/\(forall A c (H: c:* A) F U E  z q, 
+ A=(E & z ~ pos U & F) ->  E |= q :+ U -> [z ~+> q]* c :* (E&F)).
 Proof.
-  - introv Typq.
-    inductions H;introv; simpl.
+  apply typing_mut_ind.
+  - intros A a T Ok Binds F U E z q HA Typq.
+    rewrite HA in *;simpl.
     + case_var.
-      * apply binds_middle_eq_inv in H0.
-        inversion H0.
+      * apply binds_middle_eq_inv in Binds.
+        inversion Binds.
         apply_empty* typing_prf_weaken.
         assumption.
       * apply* typing_prf_var.
         apply* binds_subst.
-    + apply_fresh typing_abs.
-      rewrite* subst_open_prf_prf_var. 
-      apply_ih_bind* H0.
-    + apply_fresh typing_mu.
-      rewrite <- concat_assoc.
-      assert (y \notin L) by intuition.
-      specialize (H y H0).
-      rewrite <- concat_assoc in H.
-      destruct (typing_subst_clos (F & y~negl (neg T)) U E c z q H).
-      assumption.
-      apply* typing_closure.
-  - introv Typq.
-    inductions H;introv; simpl.
-    + apply* typing_cont_var.
-      destruct  (binds_middle_inv H0).
-      intuition.
-      destruct* H1.
-      intuition.
-      inversion H4.
-    + apply_fresh typing_mut.
-      rewrite <- concat_assoc.
-      assert (y \notin L) by intuition.
-      specialize (H y H0).
-      rewrite <- concat_assoc in H.
-      destruct* (typing_subst_clos (F & y ~ pos T) U E c z q H).
-      apply* typing_closure.
-    + apply typing_stack.
-      * apply (typing_subst_prf F U E q0 T z q H Typq).
-      * apply (typing_subst_cont F U E e (neg U0) z q H0 Typq).
-  - intro Typq.
-    inductions H;introv;simpl.
+  - intros L A U T p Hp IH F T' E z q HA Typq.
+    rewrite HA in *;simpl.
+    apply_fresh typing_abs.
+    rewrite* subst_open_prf_prf_var.
+    rewrite <- concat_assoc.
+    apply* IH.
+    rewrite* <- concat_assoc.
+  - intros L A T c Hc IH F U E z q HA Typq.
+    rewrite HA in *;simpl.
+    apply_fresh typing_mu.
+    rewrite <- concat_assoc.
+    assert (y \notin L) by intuition.
+    rewrite subst_open_clos_prf_var1.
+    + apply (IH y H _ U).
+      * rewrite* concat_assoc.
+      * assumption.
+    + apply* notin_singleton.
+    + destruct* (typing_regular_prf Typq).
+   - intros A a T Ok Binds F U E z q HA Typq.
+    rewrite HA in *;simpl.
+    apply* typing_cont_var.
+    destruct*  (binds_middle_inv Binds).
+    destruct* H.
+    intuition.
+    inversion H2.
+  - intros L A T c Hc IH F T' E z q HA Typq.
+    rewrite HA in *;simpl.
+    apply_fresh typing_mut.
+    rewrite <- concat_assoc.
+    assert (y \notin L) by intuition.
+    rewrite subst_open_clos_prf_var.
+    + apply* IH.
+      rewrite* concat_assoc.
+    + apply* notin_singleton.
+    + destruct* (typing_regular_prf Typq).
+  - intros A U T p e Hp IHp He IHe F T' E z q HA Typq.
+    rewrite HA in *;simpl.
+    apply typing_stack.
+    + apply* IHp.
+    + apply* IHe.
+  - intros A T p e Hp IHp He IHe F U E z q HA Typq.
+    rewrite HA in *;simpl.
     apply (@typing_closure (E&F) T).    
-    * apply (typing_subst_prf F U E p T z q H Typq).
-    * apply (typing_subst_cont F U E e (neg T) z q H0 Typq).
+    * apply* IHp.
+    * apply* IHe.
+Qed.
 
-Admitted.
+(* Splitting this in three pieces *)
+
+Lemma typing_prf_subst_prf:
+  forall F U E p T z q,((E & z ~ pos U & F) |= p:+ T) ->
+  E |= q :+ U -> (E & F) |= [z ~+> q]+ p :+ T.
+Proof.
+destruct typing_subst_prf as [Hp _ ].
+intros;apply* Hp.
+Qed.
+
+Lemma typing_cont_subst_prf:
+  forall F U E e T z q, (E & z ~ pos U & F) |= e:- T ->
+  E |= q :+ U -> (E & F) |= [z ~+> q]- e :- T.
+Proof.
+  destruct typing_subst_prf as [_ (He,_)].
+  intros;apply* He.
+Qed.
+  
+Lemma typing_clos_subst_prf:
+  forall F U E c z q, (c:* (E & z ~ pos U & F))->
+   E |= q :+ U -> [z ~+> q]* c :* (E&F).
+Proof.
+  destruct typing_subst_prf as [_ (_,Hc) ].
+  intros;apply* Hc.
+Qed.
+(* negative version *)
+
+Lemma typing_subst_cont:
+  (forall  A  p T (H: A |= p:+ T) F U E z f,
+     A=(E & z ~ negl (neg U) & F) -> E |= f :- neg U -> (E & F) |= [z ~-> f]+ p :+ T)
+  /\(forall A e T (H: A |= e:- T ) F U E z f,
+   A=(E & z ~ negl (neg U) & F)   ->   E |= f :- neg U -> (E & F) |= [z ~-> f]- e :- T)
+/\(forall A c (H: c:* A) F U E  z f, 
+ A=(E & z ~negl (neg U) & F) ->  E |= f :- neg U -> [z ~-> f]* c :* (E&F)).
+Proof.
+  apply typing_mut_ind.
+  - intros A a T Ok Binds F U E z q HA Typq.
+    rewrite HA in *;simpl.
+    + apply* typing_prf_var.
+      destruct* (binds_middle_inv Binds).
+      destruct* H.
+      destruct H as [_ (_,H)].
+      inversion H.
+  - intros L A U T p Hp IH F T' E z q HA Typq.
+    rewrite HA in *;simpl.
+    apply_fresh typing_abs.
+    rewrite* subst_open_prf_cont_var1.
+    rewrite <- concat_assoc.
+    apply* IH.
+    rewrite* <- concat_assoc.
+  - intros L A T c Hc IH F U E z q HA Typq.
+    rewrite HA in *;simpl.
+    apply_fresh typing_mu.
+    rewrite <- concat_assoc.
+    assert (y \notin L) by intuition.
+    rewrite subst_open_clos_cont_var.
+    + apply (IH y H _ U).
+      * rewrite* concat_assoc.
+      * assumption.
+    + apply* notin_singleton.
+    + destruct* (typing_regular_cont Typq).
+   - intros A a T Ok Binds F U E z q HA Typq.
+    rewrite HA in *;simpl.
+    case_var.
+     * apply binds_middle_eq_inv in Binds.
+       inversion Binds.
+       apply_empty* typing_cont_weaken.
+       assumption.
+     * apply* typing_cont_var.
+       apply* binds_subst.
+  - intros L A T c Hc IH F T' E z q HA Typq.
+    rewrite HA in *;simpl.
+    apply_fresh typing_mut.
+    rewrite <- concat_assoc.
+    assert (y \notin L) by intuition.
+    rewrite subst_open_clos_cont_var1.
+    + apply* IH.
+      rewrite* concat_assoc.
+    + apply* notin_singleton.
+    + destruct* (typing_regular_cont Typq).
+  - intros A U T p e Hp IHp He IHe F T' E z q HA Typq.
+    rewrite HA in *;simpl.
+    apply typing_stack.
+    + apply* IHp.
+    + apply* IHe.
+  - intros A T p e Hp IHp He IHe F U E z q HA Typq.
+    rewrite HA in *;simpl.
+    apply (@typing_closure (E&F) T).    
+    * apply* IHp.
+    * apply* IHe.
+Qed.
+
+
+
+(* Splitting this in three pieces *)
+
+Lemma typing_prf_subst_cont:
+  forall F U E p T z f,((E & z ~ negl (neg U) & F) |= p:+ T) ->
+  E |= f :- neg U -> (E & F) |= [z ~-> f]+ p :+ T.
+Proof.
+destruct typing_subst_cont as [Hp _ ].
+intros;apply* Hp.
+Qed.
+
+Lemma typing_cont_subst_cont:
+  forall F U E e T z f, (E & z ~ negl (neg U) & F) |= e:- T ->
+  E |= f :- neg U -> (E & F) |= [z ~-> f]- e :- T.
+Proof.
+  destruct typing_subst_cont as [_ (He,_)].
+  intros;apply* He.
+Qed.
+  
+Lemma typing_clos_subst_cont:
+  forall F U E c z f, (c:* (E & z ~ negl (neg U) & F))->
+   E |= f :- neg U -> [z ~-> f]* c :* (E&F).
+Proof.
+  destruct typing_subst_cont as [_ (_,Hc) ].
+  intros;apply* Hc.
+Qed.
+
+
+
 
 (** Preservation (typing is preserved by reduction). *)
 
-Lemma preservation_result : preservation.
+Lemma open_clos_comm: forall p e y,  cl p e *^+ y = cl (p+^+y) (e-^+y).
 Proof.
-  introv Typ. gen t'. inductions Typ; introv Red; inversions Red.
-  inversions Typ1. pick_fresh x. rewrite* (@subst_intro x).
-   apply_empty* typing_subst.
-  apply* typing_app. 
-  apply* typing_app.
+  intros.
+  reflexivity.
+Qed.
+
+Lemma open_cont_proof_def : forall e y, e-^+y = {0 ~+> (prf_fvar y)}-e.  
+Proof.
+  intros;reflexivity.
+Qed.
+
+Lemma subject_reduction : preservation.
+Proof.
+  introv Typ. gen c'.
+  inductions Typ;intros c Red;inversions Red.
+  - inversions H0.
+    inversion H3.
+    pick_fresh x.
+    rewrite* (@subst_intro_clos_prf x).
+    apply_empty* typing_clos_subst_prf.
+  - inversion H0.
+    apply* (@typing_closure E T0).
+    rewrite <-  H7 in *.
+    inversion H.
+    apply_fresh typing_mut.
+    simpl.
+    assert (y\notin L) by intuition.
+    rewrite open_clos_comm.
+    apply (@typing_closure (E&y~pos T0) U).
+    + apply* H13.
+    + destruct (typing_regular_cont H9).
+      rewrite open_cont_proof_def.
+      rewrite* <-(open_rec_cont_prf_id).
+      apply_empty* typing_cont_weaken.
+  - inversion H.
+    pick_fresh x.
+    rewrite* (@subst_intro_clos_cont x).
+    apply_empty* typing_clos_subst_cont.  
 Qed.
 
 (** Progress (a well-typed term is either a value or it can 
@@ -167,6 +332,7 @@ Qed.
 
 Lemma progress_result : progress.
 Proof.
+  unfold progress.
   introv Typ. lets Typ': Typ. inductions Typ.
   false* binds_empty_inv. 
   left*.
